f2effect: follow changes in store wf
Ignore-this: b161e2bad6ef03d902168aff30db597

darcs-hash:20131010100852-08f32-6dfc91f765695ed7e9e7298fef5b26f795a7cb71

done/Iron/Language/SystemF2Effect/Store/StoreP.v
@@ -3,59 +3,30 @@ Require Export Iron.Language.SystemF2Effect.Step.Frame.
 Require Export Iron.Language.SystemF2Effect.Store.Bind.
 
 
-(* All region handles on frame stack are in store properties.
+(* All region identifiers for private regions defined in the frame
+   stack are in the store properties.
 
    We don't require the other way, forcing all store properties to be in 
-   the frame stack. This is because we need to be able to pop a Use frame and
-   still have any region handles in the expression being well typed, along with
-   dangling references into that region. *)
-
+   the frame stack. This is because we need to be able to pop a Priv frame
+   and still have any region handles in the expression being well typed,
+   along with dangling references into that region. *)
 Definition STOREP  (sp : stprops) (fs : stack)
- := (forall p,     In (FPriv p)    fs -> In (SRegion p)  sp)
- /\ (forall p1 p2, In (FExt p1 p2) fs -> In (SRegion p1) sp)
- /\ (forall p1 p2, In (FExt p1 p2) fs -> In (SRegion p2) sp).
+ := (forall m1 p2, In (FPriv  m1       p2) fs -> In (SRegion p2) sp)
+ /\ (forall p1 p2, In (FPriv (Some p1) p2) fs -> In (SRegion p1) sp).
 
 
 (* Weaken frame stack in store properties. *)
 Lemma storep_snoc
  :  forall sp fs p
  ,  STOREP sp fs
- -> STOREP (SRegion p <: sp) (fs :> FPriv p).
+ -> STOREP (SRegion p <: sp) (fs :> FPriv None p).
 Proof.
  unfold STOREP in *. rip.
-
- - have HN: (p0 = p \/ ~(p0 = p)).
-   inverts HN.
-   + rrwrite (SRegion p <: sp = (SRegion p <: nil) >< sp).
-     snorm.
-   + assert (In (FPriv p0) fs).
-      eapply in_tail.
-      have (FPriv p0 <> FPriv p) by congruence.
-      eauto. auto.
-     rrwrite (SRegion p <: sp = (SRegion p <: nil) >< sp).
-     snorm.
-
- - have HN: (p1 = p \/ ~(p1 = p)).
-   inverts HN.
-   + rrwrite (SRegion p <: sp = (SRegion p <: nil) >< sp).
-     snorm.
-   + assert (In (FExt p1 p2) fs).
-      eapply in_tail.
-      have (FExt p1 p2 <> FPriv p) by congruence. 
-      eauto. auto.
-     rrwrite (SRegion p <: sp = (SRegion p <: nil) >< sp).
-     snorm. firstorder.
-  
- - have HN: (p2 = p \/ ~(p2 = p)).
-   inverts HN.
-   + rrwrite (SRegion p <: sp = (SRegion p <: nil) >< sp).
-     snorm.
-   + assert (In (FExt p1 p2) fs).
-      eapply in_tail.
-      have (FExt p1 p2 <> FPriv p) by congruence. 
-      eauto. auto.
-     rrwrite (SRegion p <: sp = (SRegion p <: nil) >< sp).
-     snorm. firstorder.
+ - inverts H0. inverts H.
+   + eauto.
+   + have HN: (p = p2 \/ ~(p = p2)).
+     inverts HN; eauto.
+ - inverts H0; nope; eauto.
 Qed.
 Hint Resolve storep_snoc.
 
@@ -65,9 +36,7 @@ Lemma storep_stprops_snoc
  ,  STOREP sp fs
  -> STOREP (p <: sp) fs.
 Proof.
- unfold STOREP in *. rip.
- - have (In (SRegion p1) sp) by firstorder. snorm.
- - have (In (SRegion p2) sp) by firstorder. snorm.
+ unfold STOREP in *. rip; eauto.
 Qed.
 Hint Resolve storep_stprops_snoc.
 
